first verion - still have errors

BPTree.dfy
@@ -5,15 +5,329 @@ class BPTree {
 
     // ghost set for verifivation
     ghost var Contents: set<int> 
-    ghost var Repr: set<BPTNode>
+    ghost var Repr: set<BPTNode> // maybe change to object, for now I think I will just have nodes in it, not this (Tree)
 
     constructor Init()
- //       ensures Well() && 
-        ensures fresh(Repr - {this})
+        ensures Well() 
+ //       ensures fresh(Repr - {this})
         ensures Contents == {}
     { 
         root := null;
-        Repr := {this};
+        Repr := {};
         Contents := {};
     } 
+
+    method Insert(val: int) // TODO: add ptrs from one leaf to another
+        requires Well()
+        modifies this, Repr
+        ensures Well()
+        ensures Contents == old(Contents) + {val}
+    {
+        if root == null { // if there was no root, root becomes leaf node with only this inserted value in it
+            root := new BPTNode.init();
+            root.keys[0] := val;
+            root.keynum := 1;
+            assert root.keynum == 1 <==> root.Contents == {root.keys[0]}; // TODO not sure if necessary 
+            assert root.well(); // TODO probably remove this from here
+        } else {
+            assert root != null;
+            var current := root;
+            var parent: BPTNode?;
+
+            assert current != null;
+
+            // reach the leaf in which we should insert value
+            while !current.is_leaf 
+                decreases current.Repr {
+                parent := current;
+
+                var i := 0;
+                while i < current.keynum {
+                    if val < current.keys[i] { // TODO be careful with < and <= signs
+                        current := current.children[i];
+                        break;
+                    }
+
+                    if i == current.keynum - 1 { // if the value is greater than all possible go to last child
+                        current := current.children[i + 1];
+                        break;
+                    }
+                    i := i + 1;
+                }
+            }
+
+            assert current.well(); // TODO do we need this?
+            assert current.is_leaf == true;
+            
+            // now we have reached leaf in which we are inserting the value 
+            if current.keynum < ORDER { // the node in which we are inserting is not full
+                var i := 0;
+                while i < current.keynum && val < current.keys[i] {
+                    i := i + 1; // find location where the value should be inserted
+                }
+
+                for j: int := current.keynum downto i {
+                    current.keys[j] := current.keys[j - 1]; // adjust other elements
+                }
+                current.keys[i] := val;
+
+                current.keynum := current.keynum + 1; // increase number of keys in the leaf
+
+                current.children[current.keynum] := current.children[current.keynum - 1]; // adjust pointer to next leaf
+                current.children[current.keynum - 1] := null;
+
+                current.Contents := current.Contents + {val}; // TODO all parents etc need to get Contents updated, maybe add while iterating or sth?
+            }
+            // not enough space in the leaf (splitting required)
+            else {  // TODO be careful here with Content and Repr, you have to move them as well
+                var newNode := new BPTNode.init();
+                var temp := new int[ORDER + 1]; // storing all keys and the new value in temporary list
+                for i := 0 to ORDER { // initialization 
+                    temp[i] := 0;
+                }
+
+                for i := 0 to ORDER { // copy all keys from the leaf (the leaf is full)
+                    temp[i] := current.keys[i];
+                }
+
+                var i := 0; // fining right position for new value
+                while val > temp[i] && i < ORDER {
+                    i := i + 1;
+                }
+
+                for j := ORDER downto i {
+                    temp[j] := temp[j - 1];
+                }
+                temp[i] := val;
+
+                // start of rearrangement 
+                current.keynum := (ORDER + 1) / 2;
+                newNode.keynum := (ORDER + 1) - (ORDER + 1) / 2;
+
+                // pointers rearrangement
+                current.children[current.keynum] := newNode;
+                newNode.children[newNode.keynum] := current.children[ORDER];
+                current.children[ORDER] := null;
+
+                current.Contents := {};
+                for i := 0 to current.keynum - 1 { 
+                    current.keys[i] := temp[i];
+                    current.Contents := current.Contents + {temp[i]}; 
+                }
+                for i := current.keynum to ORDER - 1 {
+                    current.keys[i] := 0;
+                }
+
+                var j := current.keynum;
+                for i := 0 to newNode.keynum - 1 {
+                    newNode.keys[i] := temp[j];
+                    newNode.Contents := newNode.Contents + {temp[j]}; 
+                    j := j + 1;
+                }
+            
+                assert current.is_leaf == true && newNode.is_leaf == true;
+
+                if current == root { // if current was root than we just create a new root with one key
+                    var newRoot := new BPTNode.init();
+                    newRoot.keynum := 1;
+                    newRoot.keys[0] := newNode.keys[0];
+                    newRoot.children[0] := current;
+                    newRoot.children[1] := newNode;
+                    newRoot.is_leaf := false;
+                    newRoot.Contents := newRoot.Contents + current.Contents + newNode.Contents;
+                    newRoot.Repr := newRoot.Repr + current.Repr + newNode.Repr; 
+                    root := newRoot;
+                } else { // if not, we need to update parent node
+                    ShiftLevel(newNode.keys[0], parent, newNode);
+                }
+            }
+
+        }
+
+        Contents := root.Contents;
+        Repr := root.Repr ;
+    }
+
+    method ShiftLevel(val: int, current: BPTNode, child: BPTNode) 
+    // val is value to be inserted, current is the node in which we are trying to insert and child is newly created leaf node
+        requires Well()
+        requires current.length_ok()
+        requires current.well()
+        modifies this, current, Repr
+        ensures Well()
+        decreases if root == null then {} else root.Repr - current.Repr
+    {
+        if current.keynum < ORDER { // if new key can fit into parent node (parent is not full)
+            var i := 0;
+            while i < current.keynum && val > current.keys[i] 
+                invariant 0 <= i <= current.keynum
+            {
+                i := i + 1; // find right position
+            }
+            
+            for j := current.keynum downto i {
+                current.keys[j] := current.keys[j - 1];
+            }
+
+            assert i <= current.keynum ==> (i + 1 <= current.keynum + 1);
+            for j := current.keynum + 1 downto i + 1 {
+                current.children[j] := current.children[j - 1];
+            }
+            current.keys[i] := val;
+            current.keynum := current.keynum + 1;
+            current.children[i + 1] := child;
+            current.Contents := current.Contents + {val}; // TODO this should be propagated upwards 
+            current.Repr := current.Repr + child.Repr;
+        } else { // internal node should also be splitted
+            var newInternal: BPTNode := new BPTNode.init();
+            var tempKey := new int[ORDER + 1];
+            var tempChildren := new BPTNode?[ORDER + 2];
+
+            for i := 0 to ORDER {
+                tempKey[i] := current.keys[i];
+                tempChildren[i] := current.children[i];
+            }
+            tempChildren[ORDER] := current.children[ORDER];
+
+            var i := 0;
+            while val > tempKey[i] && i < ORDER {
+                i := i + 1; // finding the right position
+            }
+
+            for j := ORDER + 1 downto i {
+                tempKey[j] := tempKey[j - 1]; 
+            }
+            tempKey[i] := val; // inserted key in its position
+            for j := ORDER + 2 downto i {
+                tempChildren[j] := tempChildren[j - 1];
+            }
+            tempChildren[i + 1] := child; // same for the pointers - new pointer in correct position
+
+            newInternal.is_leaf := false;
+            current.keynum := (ORDER + 1) / 2; // splitting the keys
+            newInternal.keynum := ORDER - (ORDER + 1) / 2;
+
+
+            // TODO -> update vrijednosti u current
+            current.Contents := {};
+            for i := 0 to current.keynum - 1 {
+                current.keys[i] := tempKey[i];
+                current.Contents := current.Contents + {tempKey[i]}; 
+            }
+            for i := current.keynum to ORDER - 1 {
+                current.keys[i] := 0; 
+            }
+
+            var j := current.keynum;
+            for i := 0 to newInternal.keynum {
+                newInternal.keys[i] := tempKey[j];
+                j := j + 1;
+            }
+            j := current.keynum + 1;
+            for i := 0 to newInternal.keynum + 1 {
+                newInternal.children[i] := tempChildren[j];
+                j := j + 1;
+            }
+
+            if current == root { // again, if previous is 
+                var newRoot := new BPTNode.init();
+                newRoot.keys[0] := newInternal.keys[0];
+                newRoot.children[0] := current;
+                newRoot.children[1] := newInternal;
+                newRoot.is_leaf := false;
+                newRoot.keynum := 1;
+                root := newRoot;
+            } else {
+                var parent := FindParent(root, current);
+                ShiftLevel(current.keys[current.keynum], parent, newInternal);
+            }
+        }
+    } 
+    
+
+    method FindParent(current: BPTNode, child: BPTNode) returns (parent: BPTNode?) 
+        requires Well()
+        requires current.well()
+        ensures Well()
+        decreases current.height
+    /* {
+        if current.is_leaf || current.children[0].is_leaf {
+            return null;
+        }
+
+        for i := 0 to current.keynum + 1 {
+            if current.children[i] == child {
+                parent := current;
+                return parent;
+            } else {
+                assert current.well() ==> current.children[i].well();
+                parent := FindParent(current.children[i], child);
+                if parent != null {
+                    return parent;
+                }
+            }
+        }
+        return null;
+    } */
+    {
+        if current.is_leaf || current.children[0].is_leaf {
+            return null;
+        }
+
+        parent := null; // Initialize parent to null
+
+        var i := 0;
+        while i <= current.keynum && parent == null 
+            decreases current.keynum - i // Ensure a decreasing loop variant
+        {
+            if current.children[i] == child {
+                parent := current;
+                return parent;
+            } else {
+                i := i + 1;
+            }
+        }
+    
+        if parent == null {
+            // If we haven't found the parent yet, continue searching in child nodes
+            i := 0;
+            while i <= current.keynum && parent == null
+                decreases current.keynum - i // Ensure a decreasing loop variant
+            {
+                assert current.children[i].well();
+                parent := FindParent(current.children[i], child);
+                i := i + 1;
+            }
+        }
+    
+        return parent;
+    }
+
+    method Main()
+        modifies this
+    {
+        // Create a new BPTree instance
+        var tree := new BPTree.Init();
+    
+        // Insert a value into the tree
+        tree.Insert(42);
+
+        // Verify that the value is in the Contents
+        assert 42 in tree.Contents;
+
+        print("Test passed: Value 42 added to the root.");
+
+    } 
+
+    ghost predicate Well()
+        reads * // TODO see if this is possible to reduce
+    {
+        // this in Repr &&
+        (root == null ==> Contents == {}) && 
+        (root != null ==> 
+            root in Repr && root.Repr <= Repr &&
+            root.well() &&
+            Contents == root.Contents)
+    }
+
 }
